imports.v
@@ -4,6 +4,6 @@ From Coq Require Export Logic.PropExtensionality
 From Equations Require Export Equations.
 From Hammer Require Export Tactics.
 From stdpp Require Export relations (rtc, rtc_transitive, rtc_once, rtc_inv, rtc(..), diamond, confluent, diamond_confluent) option (from_option).
-
+From Coq Require Export Wf_nat (well_founded_ltof, induction_ltof1).
 Require Export Psatz.
 From HB Require Export structures.
